wip

HumanEvalLean/HumanEval123.lean
@@ -2,8 +2,141 @@ import Std
 
 open Std
 
+theorem Acc.invTransGen {x y : α} (h₁ : Acc r x) (h₂ : Relation.TransGen r y x) : Acc r y := by
+  simpa [acc_transGen_iff] using h₁.transGen.inv h₂
+
+section Extrinsic
+open Relation
+
+variable {α : Sort _} {β : α → Sort _} {γ : (a : α) → β a → Sort _}
+  {C : α → Sort _} {C₂ : (a : α) → β a → Sort _} {C₃ : (a : α) → (b : β a) → γ a b → Sort _}
+
+@[inline]
+public def WellFounded.partialExtrinsicFix [∀ a, Nonempty (C a)] (R : α → α → Prop)
+    (F : ∀ a, (∀ a', R a' a → C a') → C a) (a : α) : C a :=
+  extrinsicFix (α := { a' : α // a' = a ∨ TransGen R a' a }) (C := (C ·.1))
+      (fun p q => R p.1 q.1)
+      (fun a recur => F a.1 fun a' hR => recur ⟨a', by
+        cases a.property
+        · grind [TransGen.single]
+        · apply Or.inr
+          apply TransGen.trans ?_ ‹_›
+          apply TransGen.single
+          assumption⟩ ‹_›) ⟨a, Or.inl rfl⟩
+
+public theorem WellFounded.bla {α' : Sort _} [∀ a, Nonempty (C a)] (R : α → α → Prop) (f : α' → α)
+    (F : ∀ a, (∀ a', R a' a → C a') → C a) (F' : ∀ a, (∀ a', R (f a') (f a) → C (f a')) → C (f a))
+    (h : ∀ a r, F (f a) r = F' a fun a' hR => r (f a') hR) (a : α') (h : WellFounded R) :
+    extrinsicFix (C := (C <| f ·)) (InvImage R f) F' a = extrinsicFix (C := C) R F (f a) := by
+  have h' := h
+  rcases h with ⟨h⟩
+  specialize h (f a)
+  have : Acc (InvImage R f) a := InvImage.accessible _ h
+  clear h
+  induction this
+  rename_i ih
+  rw [extrinsicFix_eq_apply, extrinsicFix_eq_apply, h]
+  · congr; ext a x
+    rw [ih _ x]
+  · assumption
+  · exact InvImage.wf _ ‹_›
+
+public theorem WellFounded.partialExtrinsicFix_eq [∀ a, Nonempty (C a)] (R : α → α → Prop)
+    (F : ∀ a, (∀ a', R a' a → C a') → C a) (a : α) (h : Acc R a) :
+    partialExtrinsicFix R F a = F a (fun a' _ => partialExtrinsicFix R F a') := by
+  simp only [partialExtrinsicFix]
+  rw [extrinsicFix_eq_apply]
+  congr; ext a' hR
+  simp
+  let f (x : { x : α // x = a' ∨ TransGen R x a' }) : { x : α // x = a ∨ TransGen R x a } :=
+    ⟨x.val, by
+      cases x.property
+      · rename_i h
+        rw [h]
+        exact Or.inr (.single hR)
+      · rename_i h
+        apply Or.inr
+        refine TransGen.trans h ?_
+        exact .single hR⟩
+  have := bla (C := (C ·.val)) (R := (R ·.1 ·.1)) (f := f) (F := fun a r => F a.1 fun a' hR => r ⟨a', Or.inr (by cases a.2; grind [TransGen.single]; exact .trans (.single hR) ‹_›)⟩ hR)
+    (F' := fun a r => F a.1 fun a' hR => r ⟨a', by cases a.2; grind [TransGen.single]; exact Or.inr (.trans (.single hR) ‹_›)⟩ hR)
+  unfold InvImage at this
+  rw [this]
+  · grind
+  · constructor
+    intro x
+    refine InvImage.accessible _ ?_
+    cases x.2 <;> rename_i hx
+    · rwa [hx]
+    · exact h.invTransGen hx
+  · constructor
+    intro x
+    refine InvImage.accessible _ ?_
+    cases x.2 <;> rename_i hx
+    · rwa [hx]
+    · exact h.invTransGen hx
+
+@[inline]
+public def WellFounded.partialExtrinsicFix₂ [∀ a b, Nonempty (C₂ a b)]
+    (R : (a : α) ×' β a → (a : α) ×' β a → Prop)
+    (F : (a : α) → (b : β a) → ((a' : α) → (b' : β a') → R ⟨a', b'⟩ ⟨a, b⟩ → C₂ a' b') → C₂ a b)
+    (a : α) (b : β a) :
+    C₂ a b :=
+  extrinsicFix₂ (α := α) (β := fun a' => { b' : β a' // (PSigma.mk a' b') = (PSigma.mk a b) ∨ TransGen R ⟨a', b'⟩ ⟨a, b⟩ })
+      (C₂ := (C₂ · ·.1))
+      (fun p q => R ⟨p.1, p.2.1⟩ ⟨q.1, q.2.1⟩)
+      (fun a b recur => F a b.1 fun a' b' hR => recur a' ⟨b', Or.inr (by
+        cases b.property
+        · grind [TransGen.single]
+        · apply TransGen.trans ?_ ‹_›
+          apply TransGen.single
+          assumption)⟩ ‹_›) a ⟨b, Or.inl rfl⟩
+
+public theorem WellFounded.partialExtrinsicFix₂_eq_partialExtrinsicFix [∀ a b, Nonempty (C₂ a b)]
+    (R : (a : α) ×' β a → (a : α) ×' β a → Prop)
+    (F : (a : α) → (b : β a) → ((a' : α) → (b' : β a') → R ⟨a', b'⟩ ⟨a, b⟩ → C₂ a' b') → C₂ a b)
+    (a : α) (b : β a) (h : Acc R ⟨a, b⟩) :
+    partialExtrinsicFix₂ R F a b = partialExtrinsicFix (α := PSigma β) (C := fun a => C₂ a.1 a.2) R (fun p r => F p.1 p.2 fun a' b' hR => r ⟨a', b'⟩ hR) ⟨a, b⟩ := by
+  simp only [partialExtrinsicFix, partialExtrinsicFix₂, extrinsicFix₂]
+  let f (x : ((a' : α) ×' { b' // PSigma.mk a' b' = ⟨a, b⟩ ∨ TransGen R ⟨a', b'⟩ ⟨a, b⟩ })) : { a' // a' = ⟨a, b⟩ ∨ TransGen R a' ⟨a, b⟩ } :=
+    ⟨⟨x.1, x.2.1⟩, x.2.2⟩
+  have := bla (C := fun a => C₂ a.1.1 a.1.2) (f := f) (R := (R ·.1 ·.1))
+    (F := fun a r => F a.1.1 a.1.2 fun a' b' hR => r ⟨⟨a', b'⟩, ?refine_a⟩ hR)
+    (F' := fun a r => F a.1 a.2.1 fun a' b' hR => r ⟨a', b', ?refine_b⟩ hR)
+    (a := ⟨a, b, ?refine_c⟩); rotate_left
+  · cases a.2 <;> rename_i heq
+    · rw [heq] at hR
+      exact .inr (.single hR)
+    · exact .inr (.trans (.single hR) heq)
+  · cases a.2.2 <;> rename_i heq
+    · rw [heq] at hR
+      exact .inr (.single hR)
+    · exact .inr (.trans (.single hR) heq)
+  · exact .inl rfl
+  unfold InvImage f at this
+  simp at this
+  rw [this]
+  constructor
+  intro x
+  apply InvImage.accessible
+  cases x.2 <;> rename_i heq
+  · rwa [heq]
+  · exact h.invTransGen heq
+
+public def WellFounded.partialExtrinsicFix₂_eq [∀ a b, Nonempty (C₂ a b)]
+    {R : (a : α) ×' β a → (a : α) ×' β a → Prop}
+    {F : (a : α) → (b : β a) → ((a' : α) → (b' : β a') → R ⟨a', b'⟩ ⟨a, b⟩ → C₂ a' b') → C₂ a b}
+    {a : α} {b : β a} (h : Acc R ⟨a, b⟩) :
+    partialExtrinsicFix₂ R F a b = F a b (fun a' b' _ => partialExtrinsicFix₂ R F a' b') := by
+  simp only [partialExtrinsicFix₂_eq_partialExtrinsicFix (h := h)]
+  rw [partialExtrinsicFix_eq (h := h)]
+  have (a' b') (hR : R ⟨a', b'⟩ ⟨a, b⟩) : Acc R ⟨a', b'⟩ := h.inv hR
+  conv => rhs; congr; intro a' b' hR; rw [partialExtrinsicFix₂_eq_partialExtrinsicFix (h := this a' b' hR)]
+
+end Extrinsic
+
 /-!
-## Preliminaries regarding termination
+## Implementation 1: no termination proof required
 -/
 
 def collatzStep (n : Nat) : Nat :=
@@ -15,6 +148,46 @@ def CollatzRel : Nat → Nat → Prop := fun m n =>
 theorem collatzRel_collatzStep {n : Nat} (h : n > 1) :
     CollatzRel (collatzStep n) n := by
   grind [CollatzRel]
+
+def oddCollatz₁ (n : Nat) : List Nat :=
+  (collectOddCollatz ⟨n, Or.inl rfl⟩ ∅).toList
+where
+  -- This function is recursive and, depending on the Collatz conjecture, it may or may not terminate.
+  -- By relying on the fixpoint combinator `extrinsicFix₂` instead of using the `partial` modifier,
+  -- we will be able to verify the function whenever the Collatz sequence terminates after
+  -- finitely many steps. A termination proof is not required for *calling* this function,
+  -- only for verifying it.
+  collectOddCollatz : (n : { m // m = n ∨ Relation.TransGen CollatzRel m n }) → (acc : TreeSet Nat compare) → TreeSet Nat compare :=
+    WellFounded.extrinsicFix₂ (CollatzRel ·.1 ·.1) fun n acc recur =>
+      if h : n.val > 1 then
+        recur ⟨collatzStep n.val, by apply Or.inr; cases n.property; rename_i h'; rw [h']; apply Relation.TransGen.single; grind [collatzRel_collatzStep]; refine Relation.TransGen.trans ?_ ‹_›; apply Relation.TransGen.single; grind [collatzRel_collatzStep]⟩
+          (if n.val % 2 = 0 then acc else acc.insert n) (by grind [CollatzRel])
+      else if n.val = 1 then
+        acc.insert 1
+      else
+        acc
+
+/-!
+## Tests 1
+-/
+
+example : oddCollatz₁ 14 = [1, 5, 7, 11, 13, 17] := by native_decide
+example : oddCollatz₁ 5 = [1, 5] := by native_decide
+example : oddCollatz₁ 12 = [1, 3, 5] := by native_decide
+example : oddCollatz₁ 1 = [1] := by native_decide
+
+/-!
+We'll verify `oddCollatz₁` after having verified `oddCollatz₂`.
+-/
+
+/-!
+## Preliminaries regarding termination
+
+Next, we provide an implementation using well-founded recursion. `oddCollatz₂ n` is guaranteed to
+terminate, but calling it requires a proof that the Collatz sequence for `n` is finite.
+In order to make this function easier to use, we start by providing a tactic that automatically
+proves the finiteness.
+-/
 
 theorem acc_collatzRel_collatzStep_iff {n : Nat} (h : n > 1) :
     Acc CollatzRel (collatzStep n) ↔ Acc CollatzRel n := by
@@ -42,13 +215,13 @@ example : (extractProof (tryDecideTermination 14 50 Iff.rfl)).isSome := by decid
 
 macro "try_decide" : tactic => `(tactic| exact ((extractProof (tryDecideTermination _ 100 Iff.rfl)).get (by decide)).down)
 
-instance : WellFoundedRelation { m : Nat // Acc CollatzRel m } := Acc.wfRel
-
 /-!
 ## Implementation
 -/
 
-def oddCollatz (n : Nat) (h : Acc CollatzRel n := by try_decide) : List Nat :=
+instance : WellFoundedRelation { m : Nat // Acc CollatzRel m } := Acc.wfRel
+
+def oddCollatz₂ (n : Nat) (h : Acc CollatzRel n := by try_decide) : List Nat :=
   (collectOddCollatz ⟨n, h⟩ ∅).toList
 where
   -- We attach a proof that `1` is reachable from `n` in finitely many steps to ensure termination.
@@ -67,12 +240,15 @@ where
 
 /-!
 ## Tests
+
+Observe that while `oddCollatz₂` is guaranteed to terminate, we do not need to manually supply
+the termination proofs. These proofs are derived automatically using the `try_decide` tactic.
 -/
 
-example : oddCollatz 14 = [1, 5, 7, 11, 13, 17] := by native_decide
-example : oddCollatz 5 = [1, 5] := by native_decide
-example : oddCollatz 12 = [1, 3, 5] := by native_decide
-example : oddCollatz 1 = [1] := by native_decide
+example : oddCollatz₂ 14 = [1, 5, 7, 11, 13, 17] := by native_decide
+example : oddCollatz₂ 5 = [1, 5] := by native_decide
+example : oddCollatz₂ 12 = [1, 3, 5] := by native_decide
+example : oddCollatz₂ 1 = [1] := by native_decide
 
 /-!
 ## Missing API
@@ -86,34 +262,31 @@ instance : LawfulOrderOrd Nat where
   isLE_compare := by grind [Nat.isLE_compare]
   isGE_compare := by grind [Nat.isGE_compare]
 
-theorem Acc.invTransGen {x y : α} (h₁ : Acc r x) (h₂ : Relation.TransGen r y x) : Acc r y := by
-  simpa [acc_transGen_iff] using h₁.transGen.inv h₂
-
 /-!
 ## Verification
 -/
 
-theorem oddCollatz_pairwise_distinct {n : Nat} {h : Acc CollatzRel n} :
-    (oddCollatz n h).Pairwise (· ≠ ·) := by
-  simpa [oddCollatz] using TreeSet.distinct_toList (α := Nat) (cmp := compare)
+theorem oddCollatz₂_pairwise_distinct {n : Nat} {h : Acc CollatzRel n} :
+    (oddCollatz₂ n h).Pairwise (· ≠ ·) := by
+  simpa [oddCollatz₂] using TreeSet.distinct_toList (α := Nat) (cmp := compare)
 
-theorem oddCollatz_pairwise_lt {n : Nat} {h : Acc CollatzRel n} :
-    (oddCollatz n h).Pairwise (· < ·) := by
-  simpa [oddCollatz, compare_eq_lt] using TreeSet.ordered_toList (α := Nat) (cmp := compare)
+theorem oddCollatz₂_pairwise_lt {n : Nat} {h : Acc CollatzRel n} :
+    (oddCollatz₂ n h).Pairwise (· < ·) := by
+  simpa [oddCollatz₂, compare_eq_lt] using TreeSet.ordered_toList (α := Nat) (cmp := compare)
 
-theorem mod_two_eq_one_of_mem_oddCollatz {m n : Nat} {h : Acc CollatzRel n} (hm : m ∈ oddCollatz n h) :
+theorem mod_two_eq_one_of_mem_oddCollatz₂ {m n : Nat} {h : Acc CollatzRel n} (hm : m ∈ oddCollatz₂ n h) :
     m % 2 = 1 := by
-  simp only [oddCollatz, TreeSet.mem_toList] at hm
+  simp only [oddCollatz₂, TreeSet.mem_toList] at hm
   generalize (⟨n, h⟩ : Subtype _) = n at hm
   generalize hg : (∅ : TreeSet Nat) = acc at hm
   have hm' (k : Nat) : k ∈ acc → k % 2 = 1 := by simp [← hg]
   clear hg
-  fun_induction oddCollatz.collectOddCollatz n acc <;> grind
+  fun_induction oddCollatz₂.collectOddCollatz n acc <;> grind
 
-theorem transGen_collatzRel_of_mem_oddCollatz {m n : Nat} {h : Acc CollatzRel n} (hm : m ∈ oddCollatz n h)
+theorem transGen_collatzRel_of_mem_oddCollatz₂ {m n : Nat} {h : Acc CollatzRel n} (hm : m ∈ oddCollatz₂ n h)
     (hne : m ≠ n) :
     Relation.TransGen CollatzRel m n := by
-  simp only [oddCollatz, TreeSet.mem_toList] at hm
+  simp only [oddCollatz₂, TreeSet.mem_toList] at hm
   generalize htmp : (⟨n, h⟩ : Subtype _) = s at hm
   rw [show n = s.val by grind] at hne ⊢
   clear htmp
@@ -123,7 +296,7 @@ theorem transGen_collatzRel_of_mem_oddCollatz {m n : Nat} {h : Acc CollatzRel n}
   generalize htmp : s = n₀ at hm' hne ⊢
   have hs : s = n₀ ∨ Relation.TransGen CollatzRel s n₀ := Or.inl htmp
   clear htmp
-  fun_induction oddCollatz.collectOddCollatz s acc
+  fun_induction oddCollatz₂.collectOddCollatz s acc
   · rename_i n' acc' h' ih
     apply ih hm
     · grind
@@ -137,47 +310,78 @@ theorem transGen_collatzRel_of_mem_oddCollatz {m n : Nat} {h : Acc CollatzRel n}
 
 theorem mem_collectOddCollatz_of_mem {n : { n : Nat // Acc CollatzRel n }} {acc : TreeSet Nat}
     {m : Nat} (h : m ∈ acc) :
-    m ∈ oddCollatz.collectOddCollatz n acc := by
-  fun_induction oddCollatz.collectOddCollatz n acc <;> grind
+    m ∈ oddCollatz₂.collectOddCollatz n acc := by
+  fun_induction oddCollatz₂.collectOddCollatz n acc <;> grind
 
 theorem mem_self_collectOddCollatz {n : { n : Nat // Acc CollatzRel n }} {acc : TreeSet Nat}
     (h : n.val % 2 = 1) :
-    n.val ∈ oddCollatz.collectOddCollatz n acc := by
-  fun_cases oddCollatz.collectOddCollatz n acc <;> grind [mem_collectOddCollatz_of_mem]
+    n.val ∈ oddCollatz₂.collectOddCollatz n acc := by
+  fun_cases oddCollatz₂.collectOddCollatz n acc <;> grind [mem_collectOddCollatz_of_mem]
 
 attribute [grind =] TreeSet.mem_toList
 
-theorem mem_self_oddCollatz {n : Nat} {h : Acc CollatzRel n} (h' : n % 2 = 1) :
-    n ∈ oddCollatz n h := by
-  grind [oddCollatz, mem_self_collectOddCollatz]
+theorem mem_self_oddCollatz₂ {n : Nat} {h : Acc CollatzRel n} (h' : n % 2 = 1) :
+    n ∈ oddCollatz₂ n h := by
+  grind [oddCollatz₂, mem_self_collectOddCollatz]
 
 theorem collectOddCollatz_mono {n : { n : Nat // Acc CollatzRel n }} {acc' acc : TreeSet Nat}
-    (h : ∀ x, x ∈ acc' → x ∈ acc) {x : Nat} (hx : x ∈ oddCollatz.collectOddCollatz n acc') :
-    x ∈ oddCollatz.collectOddCollatz n acc := by
-  fun_induction oddCollatz.collectOddCollatz n acc generalizing acc' <;>
-    grind [oddCollatz.collectOddCollatz]
+    (h : ∀ x, x ∈ acc' → x ∈ acc) {x : Nat} (hx : x ∈ oddCollatz₂.collectOddCollatz n acc') :
+    x ∈ oddCollatz₂.collectOddCollatz n acc := by
+  fun_induction oddCollatz₂.collectOddCollatz n acc generalizing acc' <;>
+    grind [oddCollatz₂.collectOddCollatz]
 
-theorem mem_oddCollatz_of_mem_oddCollatz_of_collatzRel {k m n : Nat} {hm hn}
-    (hmem : k ∈ oddCollatz m hm) (hrel : CollatzRel m n) :
-    k ∈ oddCollatz n hn := by
-  grind [oddCollatz, CollatzRel, oddCollatz.collectOddCollatz, collectOddCollatz_mono]
+theorem mem_oddCollatz₂_of_mem_oddCollatz₂_of_collatzRel {k m n : Nat} {hm hn}
+    (hmem : k ∈ oddCollatz₂ m hm) (hrel : CollatzRel m n) :
+    k ∈ oddCollatz₂ n hn := by
+  grind [oddCollatz₂, CollatzRel, oddCollatz₂.collectOddCollatz, collectOddCollatz_mono]
 
-theorem mem_oddCollatz_of_mem_oddCollatz_of_transGen {k m n : Nat} {hn}
-    (hrel : Relation.TransGen CollatzRel m n) (hmem : k ∈ oddCollatz m (hn.invTransGen hrel)) :
-    k ∈ oddCollatz n hn := by
+theorem mem_oddCollatz₂_of_mem_oddCollatz₂_of_transGen {k m n : Nat} {hn}
+    (hrel : Relation.TransGen CollatzRel m n) (hmem : k ∈ oddCollatz₂ m (hn.invTransGen hrel)) :
+    k ∈ oddCollatz₂ n hn := by
   induction hrel
-  · grind [mem_oddCollatz_of_mem_oddCollatz_of_collatzRel]
-  · grind [Acc.inv, mem_oddCollatz_of_mem_oddCollatz_of_collatzRel]
+  · grind [mem_oddCollatz₂_of_mem_oddCollatz₂_of_collatzRel]
+  · grind [Acc.inv, mem_oddCollatz₂_of_mem_oddCollatz₂_of_collatzRel]
 
-theorem mem_oddCollatz_of_transGen {m n : Nat} {hn : Acc CollatzRel n}
+theorem mem_oddCollatz₂_of_transGen {m n : Nat} {hn : Acc CollatzRel n}
     (h : Relation.TransGen CollatzRel m n) (h' : m % 2 = 1) :
-    m ∈ oddCollatz n hn := by
-  grind [mem_oddCollatz_of_mem_oddCollatz_of_transGen, mem_self_oddCollatz]
+    m ∈ oddCollatz₂ n hn := by
+  grind [mem_oddCollatz₂_of_mem_oddCollatz₂_of_transGen, mem_self_oddCollatz₂]
 
-theorem mem_oddCollatz_iff {m n : Nat} {h : Acc CollatzRel n} :
-    m ∈ oddCollatz n h ↔ m % 2 = 1 ∧ (m = n ∨ Relation.TransGen CollatzRel m n) := by
-  grind [mod_two_eq_one_of_mem_oddCollatz, transGen_collatzRel_of_mem_oddCollatz,
-    mem_self_oddCollatz, mem_oddCollatz_of_transGen]
+theorem mem_oddCollatz₂_iff {m n : Nat} {h : Acc CollatzRel n} :
+    m ∈ oddCollatz₂ n h ↔ m % 2 = 1 ∧ (m = n ∨ Relation.TransGen CollatzRel m n) := by
+  grind [mod_two_eq_one_of_mem_oddCollatz₂, transGen_collatzRel_of_mem_oddCollatz₂,
+    mem_self_oddCollatz₂, mem_oddCollatz₂_of_transGen]
+
+/-!
+## Verification 1
+-/
+
+theorem collectOddCollatz_eq_collectOddCollatz {n : Nat} {m hm'} (hn : Acc CollatzRel n) :
+    oddCollatz₁.collectOddCollatz n ⟨m, hm'⟩ acc = oddCollatz₂.collectOddCollatz ⟨m, sorry⟩ acc := by
+  rw [oddCollatz₁.collectOddCollatz]
+  have : WellFounded fun (x1 x2 : (_ : { m : Nat // m = n ∨ Relation.TransGen CollatzRel m n }) ×' TreeSet Nat) => CollatzRel x1.fst.val x2.fst.val := by
+    have := InvImage.wf (α := (_ : { m : Nat // m = n ∨ Relation.TransGen CollatzRel m n }) ×' TreeSet Nat) (β := { m : Nat // m = n ∨ Relation.TransGen CollatzRel m n }) (r := (CollatzRel ·.val ·.val)) (·.fst)
+    apply this
+    constructor
+    intro s
+    have hs : Acc CollatzRel s.val := sorry
+    apply InvImage.accessible _ hs
+  have hm : Acc CollatzRel m := sorry
+  generalize h' : (⟨m, hm⟩ : Subtype _) = s
+  have hs : s.val = n ∨ Relation.TransGen CollatzRel s.val n := by grind
+  simp only [show Subtype.mk m hm' = Subtype.mk (p := fun x => x = n ∨ Relation.TransGen CollatzRel x n) s.val hs by grind]
+  clear h'
+  rw [oddCollatz₁.collectOddCollatz, WellFounded.extrinsicFix₂_eq_fix (wf := this)]
+  fun_induction oddCollatz₂.collectOddCollatz s acc <;> grind [WellFounded.fix_eq]
+
+theorem oddCollatz₁_eq_oddCollatz₂ {n : Nat} (hn : Acc CollatzRel n) :
+    oddCollatz₁ n = oddCollatz₂ n hn := by
+  rw [oddCollatz₁, oddCollatz₂]
+  grind [collectOddCollatz_eq_collectOddCollatz]
+
+theorem mem_oddCollatz₁_iff {m n : Nat} (h : Acc CollatzRel n) :
+    m ∈ oddCollatz₁ n ↔ m % 2 = 1 ∧ (m = n ∨ Relation.TransGen CollatzRel m n) := by
+  grind [mem_oddCollatz₂_iff, oddCollatz₁_eq_oddCollatz₂]
 
 /-!
 ## Prompt
